src/parity/parity.lean
@@ -16,29 +16,29 @@ open nat list
 open encoding
 
 -- Represents the type of the variable stored in the literal
-variables {V : Type u} [decidable_eq V]
+variables {V : Type*} [decidable_eq V]
 
 /- An n-variable XOR constraint is a map from a list of bools to an output bool -/
-def Xor : constraint := λ l, (l.foldr bxor ff)
-def XorF : constraint := λ l, (l.foldr bxor tt)
+def parity : constraint := λ l, (l.foldr bxor ff)
+def parityF : constraint := λ l, (l.foldr bxor tt)
 
-namespace Xor
+namespace parity
 
 /-! # eval -/
 section eval
 
 variables (τ : assignment V) (l l₁ l₂ : list (literal V)) (lit : literal V)
 
-@[simp] theorem eval_nil : Xor.eval τ [] = ff := rfl
+@[simp] theorem eval_nil : parity.eval τ [] = ff := rfl
 
-@[simp] theorem eval_singleton : Xor.eval τ [lit] = lit.eval τ :=
-by simp only [constraint.eval, Xor, map, bool.bxor_ff_right, foldr]
+@[simp] theorem eval_singleton : parity.eval τ [lit] = lit.eval τ :=
+by simp only [constraint.eval, parity, map, bool.bxor_ff_right, foldr]
 
-theorem eval_cons : Xor.eval τ (lit :: l) = bxor (lit.eval τ) (Xor.eval τ l) :=
-by simp only [constraint.eval, Xor, foldr, foldr_map]
+theorem eval_cons : parity.eval τ (lit :: l) = bxor (lit.eval τ) (parity.eval τ l) :=
+by simp only [constraint.eval, parity, foldr, foldr_map]
 
 theorem eval_append : 
-  Xor.eval τ (l₁ ++ l₂) = bxor (Xor.eval τ l₁) (Xor.eval τ l₂) :=
+  parity.eval τ (l₁ ++ l₂) = bxor (parity.eval τ l₁) (parity.eval τ l₂) :=
 begin
   induction l₁ with l ls ih,
   { simp only [bool.bxor_ff_left, eval_nil, nil_append] },
@@ -46,15 +46,15 @@ begin
 end
 
 /- Evaluates to true if an odd number of literals evaluates to true -/
-theorem eval_eq_bodd_count_tt : Xor.eval τ l = bodd (clause.count_tt τ l) :=
+theorem eval_eq_bodd_count_tt : parity.eval τ l = bodd (clause.count_tt τ l) :=
 begin
   induction l with l ls ih,
   { simp only [bodd_zero, eval_nil, count_tt_nil] },
-  { cases h : (l.eval τ); { simp [Xor.eval_cons, count_tt_cons, h, ih] } }
+  { cases h : (l.eval τ); { simp [parity.eval_cons, count_tt_cons, h, ih] } }
 end
 
 theorem eval_eq_of_perm {l₁ l₂ : list (literal V)} : l₁ ~ l₂ → 
-  ∀ (τ : assignment V), Xor.eval τ l₁ = Xor.eval τ l₂ :=
+  ∀ (τ : assignment V), parity.eval τ l₁ = parity.eval τ l₂ :=
 begin
   intros hp τ,
   induction hp with x l₂ l₂' p IH  x y l₂  l₂ m₂ r₂ p₁ p₂ IH₁ IH₂,
@@ -67,17 +67,17 @@ end
 
 open assignment
 
-theorem eval_eq_of_eqod [decidable_eq V] {τ₁ τ₂ : assignment V} {l : list (literal V)} :
-  (eqod τ₁ τ₂ (clause.vars l)) → Xor.eval τ₁ l = Xor.eval τ₂ l :=
+theorem eval_eq_of_agree_on [decidable_eq V] {τ₁ τ₂ : assignment V} {l : list (literal V)} :
+  (agree_on τ₁ τ₂ (clause.vars l)) → parity.eval τ₁ l = parity.eval τ₂ l :=
 begin
   induction l with l ls ih,
-  { simp only [eqod_nil, Xor.eval_nil, forall_true_left, clause.vars_nil] },
+  { simp only [agree_on_nil, parity.eval_nil, forall_true_left, clause.vars_nil] },
   { intro h,
-    simp only [Xor.eval_cons],
-    rw eval_eq_of_eqod_of_var_mem h (mem_vars_of_mem (mem_cons_self l ls)),
-    rw ih (eqod_subset (vars_subset_of_vars_cons l ls) h) }
+    simp only [parity.eval_cons],
+    rw eval_eq_of_agree_on_of_var_mem h (mem_vars_of_mem (mem_cons_self l ls)),
+    rw ih (agree_on_subset (vars_subset_of_vars_cons l ls) h) }
 end
 
 end eval
 
-end Xor
+end parity
