src/parity/recursive_parity.lean
@@ -1,6 +1,6 @@
 /-
-This file contains the Tseitin encoding for XOR.
-Both the pooled and linear encodigns are included here.
+This file contains the recursive encoding for parity.
+Both the pooled and linear encodings are included here.
 
 Authors: Cayden Codel, Jeremy Avidgad, Marijn Heule
 Carnegie Mellon University
@@ -11,18 +11,18 @@ import cnf.clause
 import cnf.cnf
 import cnf.encoding
 import cnf.gensym
-import xor.xor
-import xor.direct_xor
+import parity.parity
+import parity.direct_parity
 
 import data.list.basic
 import data.nat.basic
 
 variables {V : Type*} [inhabited V] [decidable_eq V]
 
-open literal clause cnf Xor encoding gensym assignment
+open literal clause cnf parity encoding gensym assignment
 open nat list list.perm function
 
-namespace tseitin_xor
+namespace recursive_parity
 
 variables {l : list (literal V)} {g : gensym V} {k : nat} (hk : k ≥ 3) {v : V} {τ : assignment V}
 
@@ -53,57 +53,57 @@ end
 
 variables {p : list (literal V) → list (literal V)} (hp : ∀ l, perm l (p l))
 
-def tseitin_xor : encoding V 
+def recursive_parity : enc_fn V 
 | l g :=  if h : length l ≤ k then direct_xor l g else
     have length (p (Pos g.fresh.1 :: (l.drop (k - 1)))) < length l,
       from (perm.length_eq (hp (Pos g.fresh.1 :: (l.drop (k - 1))))) ▸ 
              (drop_len_lt _ hk (not_le.mp h)),
     ⟨(direct_xor (l.take (k - 1) ++ [(Neg g.fresh.1)]) g.fresh.2).1 ++
-     (tseitin_xor (p (Pos g.fresh.1 :: (l.drop (k - 1)))) g.fresh.2).1,
-     (tseitin_xor (p (Pos g.fresh.1 :: (l.drop (k - 1)))) g.fresh.2).2⟩ 
+     (recursive_parity (p (Pos g.fresh.1 :: (l.drop (k - 1)))) g.fresh.2).1,
+     (recursive_parity (p (Pos g.fresh.1 :: (l.drop (k - 1)))) g.fresh.2).2⟩ 
 using_well_founded {
   rel_tac := λ a b, `[exact ⟨_, measure_wf (λ σ, list.length σ.1)⟩],
   dec_tac := tactic.assumption
 }
 
-def tseitin_xor' : encoding V 
+def recursive_parity' : enc_fn V 
 | l g :=  if h : length l ≤ k then direct_xor l g else
     let ⟨y, g₁⟩ := g.fresh in
     have length (p (Pos y :: (l.drop (k - 1)))) < length l,
       from (perm.length_eq (hp (Pos y :: (l.drop (k - 1))))) ▸ 
            (drop_len_lt _ hk (not_le.mp h)),
-    let ⟨Frec, g₂⟩ := tseitin_xor' (p (Pos y :: (l.drop (k - 1)))) g₁ in
+    let ⟨Frec, g₂⟩ := recursive_parity' (p (Pos y :: (l.drop (k - 1)))) g₁ in
       ⟨(direct_xor (l.take (k - 1) ++ [Neg y]) g₁).1 ++ Frec, g₂⟩
 using_well_founded {
   rel_tac := λ a b, `[exact ⟨_, measure_wf (λ σ, list.length σ.1)⟩],
   dec_tac := tactic.assumption
 }
 
-theorem tseitin_xor_eq_tseitin_xor' : ∀ (l : list (literal V)) (g : gensym V),
-  tseitin_xor hk hp l g = tseitin_xor' hk hp l g :=
+theorem recursive_parity_eq_recursive_parity' : ∀ (l : list (literal V)) (g : gensym V),
+  recursive_parity hk hp l g = recursive_parity' hk hp l g :=
 begin
   intros l g,
   induction l using strong_induction_on_lists with l ih generalizing g,
-  rw [tseitin_xor, tseitin_xor'],
+  rw [recursive_parity, recursive_parity'],
   by_cases hl : length l ≤ k,
   { simp [hl] },
   { simp [hl, fresh],
-    rw [tseitin_xor'._match_2, prod.ext_self (tseitin_xor' hk hp _ _), ← ih, tseitin_xor'._match_1],
+    rw [recursive_parity'._match_2, prod.ext_self (recursive_parity' hk hp _ _), ← ih, recursive_parity'._match_1],
     exact (perm.length_eq (hp (Pos g.fresh.1 :: (l.drop (k - 1))))) ▸ 
              (drop_len_lt _ hk (not_le.mp hl)) }
 end
 
-lemma tseitin_base_case : length l ≤ k → (tseitin_xor hk hp l g).1 = (direct_xor l g).1 :=
-assume h, by { rw tseitin_xor, simp only [h, if_true] }
+lemma tseitin_base_case : length l ≤ k → (recursive_parity hk hp l g).1 = (direct_xor l g).1 :=
+assume h, by { rw recursive_parity, simp only [h, if_true] }
 
-theorem mem_tseitin_xor_vars_of_mem_vars (hdis : disj l g) :
-  clause.vars l ⊆ (tseitin_xor hk hp l g).1.vars :=
+theorem mem_recursive_parity_vars_of_mem_vars (hdis : disj l g) :
+  clause.vars l ⊆ (recursive_parity hk hp l g).1.vars :=
 begin
   induction l using strong_induction_on_lists with l ih generalizing g,
   by_cases hl : length l ≤ k,
   { rw [tseitin_base_case hk hp hl, ← direct_xor_eq_direct_xor, vars_direct_xor], refl },
   { intros v hv,
-    rw tseitin_xor,
+    rw recursive_parity,
     simp [hl],
     rw [← take_append_drop (k - 1) l, clause.vars_append] at hv,
     rcases finset.mem_union.mp hv with (h | h),
@@ -120,13 +120,13 @@ begin
       exact or.inr (this (mem_vars_cons_of_mem_vars _ h)) } }
 end
 
-theorem tseitin_xor_is_wb : is_wb (tseitin_xor hk hp) :=
+theorem recursive_parity_is_wb : is_wb (recursive_parity hk hp) :=
 begin
   intros l g hdis,
   induction l using strong_induction_on_lists with l ih generalizing g,
-  rw tseitin_xor,
+  rw recursive_parity,
   by_cases hl : length l ≤ k,
-  { simp [hl], exact (direct_xor_encodes_Xor.2 hdis) },
+  { simp [hl], exact (direct_xor_encodes_parity.2 hdis) },
   { simp [hl],
     have h₁ := drop_len_lt (Pos g.fresh.1) hk (not_le.mp hl),
     rw perm.length_eq (hp (Pos g.fresh.1 :: drop (k - 1) l)) at h₁,
@@ -161,14 +161,14 @@ begin
 end
 
 -- TODO: make into a shorter lemma
-theorem not_mem_tseitin_xor_vars_of_not_mem_vars_of_not_mem_stock (hdis : disj l g) :
-  v ∉ (clause.vars l) → v ∉ g.stock → v ∉ (tseitin_xor hk hp l g).1.vars :=
+theorem not_mem_recursive_parity_vars_of_not_mem_vars_of_not_mem_stock (hdis : disj l g) :
+  v ∉ (clause.vars l) → v ∉ g.stock → v ∉ (recursive_parity hk hp l g).1.vars :=
 begin
   induction l using strong_induction_on_lists with l ih generalizing g,
   by_cases hl : length l ≤ k,
   { rw [tseitin_base_case hk hp hl, ← direct_xor_eq_direct_xor, vars_direct_xor l], tautology },
   { intros hvars hg,
-    rw tseitin_xor,
+    rw recursive_parity,
     simp [hl, not_or_distrib],
     split,
     { rw [← direct_xor_eq_direct_xor, vars_direct_xor, clause.vars_append],
@@ -195,14 +195,14 @@ begin
 end
 
 lemma tseitin_reverse (hdis : disj l g) :
-  (tseitin_xor hk hp l g).1.eval τ = tt → Xor.eval τ l = tt :=
+  (recursive_parity hk hp l g).1.eval τ = tt → parity.eval τ l = tt :=
 begin
   intro he,
   induction l using strong_induction_on_lists with l ih generalizing g,
   by_cases hl : length l ≤ k,
-  { rw [tseitin_base_case hk hp hl, ← direct_xor_eq_direct_xor, eval_direct_xor_eq_eval_Xor] at he,
+  { rw [tseitin_base_case hk hp hl, ← direct_xor_eq_direct_xor, eval_direct_xor_eq_eval_parity] at he,
     exact he },
-  { rw tseitin_xor at he,
+  { rw recursive_parity at he,
     simp [hl, cnf.eval_append] at he,
     rcases he with ⟨hdir, hrec⟩,
     have h₁ := drop_len_lt (Pos g.fresh.1) hk (not_le.mp hl),
@@ -210,7 +210,7 @@ begin
     rw perm.length_eq (hp (Pos g.fresh.1 :: drop (k - 1) l)) at h₁,
     rw (disj_perm hp) at h₂,
     have ihred := ih _ h₁ h₂ hrec,
-    rw [← direct_xor_eq_direct_xor, eval_direct_xor_eq_eval_Xor] at hdir,
+    rw [← direct_xor_eq_direct_xor, eval_direct_xor_eq_eval_parity] at hdir,
     rw eval_eq_bodd_count_tt at ihred hdir |-,
     rw ← clause.count_tt_perm (hp (Pos g.fresh.1 :: drop (k - 1) l)) at ihred,
     have := congr_arg ((clause.count_tt τ)) (take_append_drop (k - 1) l).symm,
@@ -224,20 +224,20 @@ begin
       exact this } }
 end
 
-theorem tseitin_xor_encodes_Xor : encodes Xor (tseitin_xor hk hp) :=
+theorem recursive_parity_encodes_parity : encodes parity (recursive_parity hk hp) :=
 begin
   split,
   { intros l g hdis τ,
     induction l using strong_induction_on_lists with l ih generalizing g τ,
     by_cases hl : length l ≤ k,
     { rw tseitin_base_case hk hp hl,
-      exact direct_xor_formula_encodes_Xor l τ },
+      exact direct_xor_formula_encodes_parity l τ },
     { have h₁ := drop_len_lt (Pos g.fresh.1) hk (not_le.mp hl),
       rw perm.length_eq (hp (Pos g.fresh.1 :: drop (k - 1) l)) at h₁,
       have h₂ := disjoint_fresh_of_disjoint k hdis,
       rw (disj_perm hp) at h₂,
       split,
-      { rw tseitin_xor,
+      { rw recursive_parity,
         simp [hl],
         have hnotmem := set.disjoint_left.mp hdis (g.fresh_mem_stock),
         have htakevars := vars_subset_of_subset (take_subset (k - 1) l),
@@ -246,21 +246,21 @@ begin
         rw [eval_eq_bodd_count_tt, ← (take_append_drop (k - 1) l), clause.count_tt_append, bodd_add] at heval,
         cases hevalsub : bodd (clause.count_tt τ (take (k - 1) l)),
         { rw [hevalsub, bool.bxor_ff_left] at heval,
-          rcases exists_eqod_and_eq_of_not_mem τ ff hnotmem with ⟨γ, heqod, hg⟩,
+          rcases exists_agree_on_and_eq_of_not_mem τ ff hnotmem with ⟨γ, hagree_on, hg⟩,
           have : bodd (clause.count_tt γ (Pos g.fresh.1 :: drop (k - 1) l)) = tt,
           { simp only [clause.count_tt_cons, literal.eval, hg, cond,
-              ← count_tt_eq_of_eqod (eqod_subset hdropvars heqod), heval] },
+              ← count_tt_eq_of_agree_on (agree_on_subset hdropvars hagree_on), heval] },
           rw [← eval_eq_bodd_count_tt, eval_eq_of_perm (hp (Pos g.fresh.1 :: drop (k - 1) l))] at this,
 
           -- Apply the induction hypothesis
           rcases (ih _ h₁ _ h₂).mp this with ⟨γ₂, he₂, hg₂⟩,
 
-          have heqod₂ : eqod (assignment.ite ((tseitin_xor hk hp (p (Pos g.fresh.1 :: (l.drop (k - 1)))) g.fresh.2).1.vars) γ₂ γ) γ (clause.vars l),
+          have hagree_on₂ : agree_on (aite ((recursive_parity hk hp (p (Pos g.fresh.1 :: (l.drop (k - 1)))) g.fresh.2).1.vars) γ₂ γ) γ (clause.vars l),
           { intros v hv,
             by_cases hmem : v ∈ clause.vars (l.drop (k - 1)),
             { have h₃ := mem_vars_cons_of_mem_vars (Pos g.fresh.1) hmem,
               rw vars_perm (hp (Pos g.fresh.1 :: drop (k - 1) l)) at h₃,
-              rw [ite_pos (mem_tseitin_xor_vars_of_mem_vars hk hp h₂ h₃), hg₂ v h₃] },
+              rw [aite_pos (mem_recursive_parity_vars_of_mem_vars hk hp h₂ h₃), hg₂ v h₃] },
             { have hdis₂ := set.disjoint_right.mp hdis hv,
               have hne : v ≠ g.fresh.1,
               { exact (λ hcon, (hcon ▸ hdis₂) (fresh_mem_stock g)) },
@@ -272,40 +272,40 @@ begin
               rw vars_perm (hp (Pos g.fresh.1 :: drop (k - 1) l)) at this,
               have hstock : v ∉ g.fresh.2.stock,
               { exact (λ hcon, hdis₂ ((fresh_stock_subset g) hcon)) },
-              rw ite_neg (not_mem_tseitin_xor_vars_of_not_mem_vars_of_not_mem_stock hk hp h₂ this hstock) } },
+              rw aite_neg (not_mem_recursive_parity_vars_of_not_mem_vars_of_not_mem_stock hk hp h₂ this hstock) } },
 
-          use assignment.ite (tseitin_xor hk hp (p (Pos g.fresh.1 :: (l.drop (k - 1)))) g.fresh.2).1.vars γ₂ γ,
+          use aite (recursive_parity hk hp (p (Pos g.fresh.1 :: (l.drop (k - 1)))) g.fresh.2).1.vars γ₂ γ,
           split,
           { split,
             { rw ← direct_xor_eq_direct_xor,
-              simp [eval_direct_xor_eq_eval_Xor, eval_eq_bodd_count_tt, 
+              simp [eval_direct_xor_eq_eval_parity, eval_eq_bodd_count_tt, 
               clause.count_tt_append, bodd_add, literal.eval, hg],
               have : g.fresh.1 ∈ clause.vars (Pos g.fresh.1 :: (l.drop (k - 1))),
               { exact mem_vars_cons_self _ _ },
               rw vars_perm (hp (Pos g.fresh.1 :: drop (k - 1) l)) at this,
-              simp [ite_pos (mem_tseitin_xor_vars_of_mem_vars hk hp h₂ this), 
+              simp [aite_pos (mem_recursive_parity_vars_of_mem_vars hk hp h₂ this), 
                 ← (hg₂ g.fresh.1 this), hg,
-                count_tt_eq_of_eqod (eqod_subset htakevars heqod₂),
-                ← count_tt_eq_of_eqod (eqod_subset htakevars heqod), hevalsub] },
-            { exact he₂ ▸ eval_eq_of_eqod (ite_eqod _ _ _) } },
-          { exact eqod.trans heqod (heqod₂.symm) } },
+                count_tt_eq_of_agree_on (agree_on_subset htakevars hagree_on₂),
+                ← count_tt_eq_of_agree_on (agree_on_subset htakevars hagree_on), hevalsub] },
+            { exact he₂ ▸ eval_eq_of_agree_on (aite_agree_on _ _ _) } },
+          { exact agree_on.trans hagree_on (hagree_on₂.symm) } },
         { simp only [hevalsub, bnot_eq_true_eq_eq_ff, tt_bxor] at heval,
-          rcases exists_eqod_and_eq_of_not_mem τ tt hnotmem with ⟨γ, heqod, hg⟩,
+          rcases exists_agree_on_and_eq_of_not_mem τ tt hnotmem with ⟨γ, hagree_on, hg⟩,
           have : bodd (clause.count_tt γ (Pos g.fresh.1 :: drop (k - 1) l)) = tt,
           { simp only [clause.count_tt_cons, literal.eval, hg, cond, 
-              ← count_tt_eq_of_eqod (eqod_subset hdropvars heqod), heval, bodd_succ,
+              ← count_tt_eq_of_agree_on (agree_on_subset hdropvars hagree_on), heval, bodd_succ,
               bodd_add, bodd_zero, bool.bnot_ff, bxor_tt_left], },
           rw [← eval_eq_bodd_count_tt, eval_eq_of_perm (hp (Pos g.fresh.1 :: drop (k - 1) l))] at this,
 
           -- Apply the induction hypothesis
           rcases (ih _ h₁ _ h₂).mp this with ⟨γ₂, he₂, hg₂⟩,
 
-          have heqod₂ : eqod (assignment.ite (tseitin_xor hk hp (p (Pos g.fresh.1 :: (l.drop (k - 1)))) g.fresh.2).1.vars γ₂ γ) γ (clause.vars l),
+          have hagree_on₂ : agree_on (aite (recursive_parity hk hp (p (Pos g.fresh.1 :: (l.drop (k - 1)))) g.fresh.2).1.vars γ₂ γ) γ (clause.vars l),
           { intros v hv,
             by_cases hmem : v ∈ clause.vars (l.drop (k - 1)),
             { have h₃ := mem_vars_cons_of_mem_vars (Pos g.fresh.1) hmem,
               rw vars_perm (hp (Pos g.fresh.1 :: drop (k - 1) l)) at h₃,
-              rw [ite_pos (mem_tseitin_xor_vars_of_mem_vars hk hp h₂ h₃), hg₂ v h₃] },
+              rw [aite_pos (mem_recursive_parity_vars_of_mem_vars hk hp h₂ h₃), hg₂ v h₃] },
             { have hdis₂ := set.disjoint_right.mp hdis hv,
               have hne : v ≠ g.fresh.1,
               { exact (λ hcon, (hcon ▸ hdis₂) (fresh_mem_stock g)) },
@@ -317,41 +317,40 @@ begin
               rw vars_perm (hp (Pos g.fresh.1 :: drop (k - 1) l)) at this,
               have hstock : v ∉ g.fresh.2.stock,
               { exact (λ hcon, hdis₂ ((fresh_stock_subset g) hcon)) },
-              rw ite_neg (not_mem_tseitin_xor_vars_of_not_mem_vars_of_not_mem_stock hk hp h₂ this hstock) } },
+              rw aite_neg (not_mem_recursive_parity_vars_of_not_mem_vars_of_not_mem_stock hk hp h₂ this hstock) } },
           
-          use assignment.ite (tseitin_xor hk hp (p (Pos g.fresh.1 :: (l.drop (k - 1)))) g.fresh.2).1.vars γ₂ γ,
+          use aite (recursive_parity hk hp (p (Pos g.fresh.1 :: (l.drop (k - 1)))) g.fresh.2).1.vars γ₂ γ,
           split,
           { split,
             { rw ← direct_xor_eq_direct_xor,
-              simp [eval_direct_xor_eq_eval_Xor, eval_eq_bodd_count_tt, 
+              simp [eval_direct_xor_eq_eval_parity, eval_eq_bodd_count_tt, 
                 clause.count_tt_append, bodd_add, literal.eval, hg],
               have : g.fresh.1 ∈ clause.vars (Pos g.fresh.1 :: (l.drop (k - 1))),
               { exact mem_vars_cons_self _ _ },
               rw vars_perm (hp (Pos g.fresh.1 :: drop (k - 1) l)) at this,
-              simp [ite_pos (mem_tseitin_xor_vars_of_mem_vars hk hp h₂ this), 
+              simp [aite_pos (mem_recursive_parity_vars_of_mem_vars hk hp h₂ this), 
                 ← (hg₂ g.fresh.1 this), hg,
-                count_tt_eq_of_eqod (eqod_subset htakevars heqod₂),
-                ← count_tt_eq_of_eqod (eqod_subset htakevars heqod), hevalsub] },
-            { exact he₂ ▸ eval_eq_of_eqod (ite_eqod _ _ _) } },
-        { exact eqod.trans heqod heqod₂.symm } } },
-      { rintros ⟨σ, heval, heqod⟩,
-        rw Xor.eval_eq_of_eqod heqod,
+                count_tt_eq_of_agree_on (agree_on_subset htakevars hagree_on₂),
+                ← count_tt_eq_of_agree_on (agree_on_subset htakevars hagree_on), hevalsub] },
+            { exact he₂ ▸ eval_eq_of_agree_on (aite_agree_on _ _ _) } },
+        { exact agree_on.trans hagree_on hagree_on₂.symm } } },
+      { rintros ⟨σ, heval, hagree_on⟩,
+        rw parity.eval_eq_of_agree_on hagree_on,
         exact tseitin_reverse hk hp hdis heval } } },
-  { exact tseitin_xor_is_wb hk hp }
+  { exact recursive_parity_is_wb hk hp }
 end
 
 def linear_perm (l : list (literal V)) : list (literal V) := l
 
 lemma linear_perm_is_perm : ∀ (l : list (literal V)), l ~ linear_perm l :=
 begin
-  intro l,
-  rw linear_perm
+  intro l, rw linear_perm
 end
 
-def linear_xor : encoding V := tseitin_xor hk linear_perm_is_perm
+def linear_parity : enc_fn V := recursive_parity hk linear_perm_is_perm
 
-theorem linear_xor_encodes_Xor : encodes Xor (linear_xor hk : encoding V) :=
-tseitin_xor_encodes_Xor hk linear_perm_is_perm
+theorem linear_parity_encodes_parity : encodes parity (linear_parity hk : enc_fn V) :=
+recursive_parity_encodes_parity hk linear_perm_is_perm
 
 def pooled_perm : list (literal V) → list (literal V)
 | []        := []
@@ -366,9 +365,9 @@ begin
     exact perm_append_comm }
 end
 
-def pooled_xor : encoding V := tseitin_xor hk pooled_perm_is_perm
+def pooled_parity : enc_fn V := recursive_parity hk pooled_perm_is_perm
 
-theorem pooled_xor_encodes_Xor : encodes Xor (pooled_xor hk : encoding V) :=
-tseitin_xor_encodes_Xor hk pooled_perm_is_perm
+theorem pooled_parity_encodes_parity : encodes parity (pooled_parity hk : enc_fn V) :=
+recursive_parity_encodes_parity hk pooled_perm_is_perm
 
-end tseitin_xor
+end recursive_parity
